proof/crefine/RISCV64/ADT_C.thy
@@ -294,11 +294,13 @@ lemma cirqstate_cancel:
 
 definition
   "cint_state_to_H cnode cirqs \<equiv>
-   InterruptState (ptr_val cnode)
-     (\<lambda>i::6 word. if i \<le> maxIRQ then cirqstate_to_H (index cirqs (unat i))
-                else irqstate.IRQInactive)"
+     InterruptState (ptr_val cnode)
+       (\<lambda>i::irq. if i \<le> maxIRQ then cirqstate_to_H (index cirqs (unat i))
+                 else irqstate.IRQInactive)"
 
-lemma cint_rel_to_H:
+end
+
+lemma (in kernel_m) cint_rel_to_H:
   "irqs_masked' s \<Longrightarrow>
    cinterrupt_relation (ksInterruptState s) n t \<Longrightarrow>
    cint_state_to_H n t = (ksInterruptState s)"
@@ -306,9 +308,9 @@ lemma cint_rel_to_H:
   apply (cases "ksInterruptState s")
   apply (rename_tac "fun")
   apply (clarsimp simp: cinterrupt_relation_def cint_state_to_H_def
-                        maxIRQ_def Kernel_C.maxIRQ_def)
+                        maxIRQ_def Kernel_C_maxIRQ)
   apply (rule ext)
-  apply clarsimp
+  apply (clarsimp split: if_split)
   apply (drule spec, erule impE, assumption)
   apply (drule_tac s="irqstate_to_C (fun i)" in sym,
          simp add: cirqstate_cancel[THEN fun_cong, simplified])
@@ -321,6 +323,8 @@ definition
 lemma projectKO_opt_UserData [simp]:
   "projectKO_opt KOUserData = Some UserData"
   by (simp add: projectKO_opts_defs)
+
+context begin interpretation Arch . (*FIXME: arch-split*)
 
 lemma ucast_ucast_mask_pageBits_shift:
   "ucast (ucast (p && mask pageBits >> 3) :: 9 word) = p && mask pageBits >> 3"
